Work on a fix

backend/Tailcallproof.v
@@ -428,35 +428,36 @@ We first define the simulation invariant between call stacks.
 The first two cases are standard, but the third case corresponds
 to a frame that was eliminated by the transformation. *)
 
-Inductive match_stackframes (m: mem): compartment -> list stackframe -> list stackframe -> Prop :=
-  | match_stackframes_nil: forall cp,
-      match_stackframes m cp nil nil
-  | match_stackframes_normal: forall stk stk' res sp pc rs rs' ce f cp,
-      match_stackframes m (comp_of f) stk stk' ->
+Inductive match_stackframes (m: mem): list stackframe -> list stackframe -> Prop :=
+  | match_stackframes_nil: (* forall cp, *)
+      match_stackframes m (* cp *) nil nil
+  | match_stackframes_normal: forall stk stk' res sp pc rs rs' ce f (* cp *),
+      match_stackframes m (* (comp_of f) *) stk stk' ->
       forall (COMPAT: cenv_compat prog ce),
       forall (UPD: uptodate_caller (comp_of f) (call_comp stk) (call_comp stk')),
       forall (ACC: Mem.can_access_block m sp (Some (comp_of f))),
       regs_lessdef rs rs' ->
-      match_stackframes m cp
+      match_stackframes m (* cp *)
         (Stackframe res f (Vptr sp Ptrofs.zero) pc rs :: stk)
         (Stackframe res (transf_function ce f) (Vptr sp Ptrofs.zero) pc rs' :: stk')
   | match_stackframes_tail: forall stk stk' res sp pc rs f,
-      match_stackframes m (comp_of f) stk stk' ->
+      match_stackframes m (* (comp_of f) *) stk stk' ->
       is_return_spec f pc res ->
       f.(fn_stacksize) = 0 ->
-      (* comp_of f = call_comp stk -> *)
-      match_stackframes m (comp_of f)
+      match_stackframes m (* (comp_of f) *)
         (Stackframe res f (Vptr sp Ptrofs.zero) pc rs :: stk)
         stk'.
 
 (* Lemma match_stackframes_call_comp: forall m cp stk stk', *)
 (*     match_stackframes m cp stk stk' -> *)
-(*     call_comp stk = call_comp stk'. *)
+(*     (call_comp stk <> cp -> call_comp stk = call_comp stk'). *)
+(*     (* call_comp stk = call_comp stk'. *) *)
 (* Proof. *)
 (*   induction 1. *)
 (*   - reflexivity. *)
 (*   - simpl; rewrite comp_transf_function; reflexivity. *)
-(*   - simpl. congruence. *)
+(*   - simpl. intros. congruence. *)
+(*     (* specialize (IHmatch_stackframes H2). congruence. *) *)
 (* Qed. *)
 
 
@@ -468,7 +469,7 @@ Inductive match_stackframes (m: mem): compartment -> list stackframe -> list sta
 Inductive match_states: state -> state -> Prop :=
   | match_states_normal:
       forall s sp pc rs m s' rs' m' ce f
-             (STACKS: match_stackframes m' (comp_of f) s s')
+             (STACKS: match_stackframes m' (* (comp_of f) *) s s')
              (COMPAT: cenv_compat prog ce)
              (RLD: regs_lessdef rs rs')
              (MLD: Mem.extends m m')
@@ -478,7 +479,7 @@ Inductive match_states: state -> state -> Prop :=
                    (State s' (transf_function ce f) (Vptr sp Ptrofs.zero) pc rs' m')
   | match_states_call:
       forall s ce f args m s' args' m',
-      match_stackframes m' (comp_of f) s s' ->
+      match_stackframes m' (* (comp_of f) *) s s' ->
       forall (COMPAT: cenv_compat prog ce),
       forall (UPD: uptodate_caller (comp_of f) (call_comp s) (call_comp s')),
       Val.lessdef_list args args' ->
@@ -486,21 +487,33 @@ Inductive match_states: state -> state -> Prop :=
       match_states (Callstate s f args m)
                    (Callstate s' (transf_fundef ce f) args' m')
   | match_states_return:
-      forall s v m s' v' m' cp,
-      match_stackframes m' cp s s' ->
+      forall s v m s' v' m' (* cp *),
+      match_stackframes m' (* cp *) s s' ->
       Val.lessdef v v' ->
       Mem.extends m m' ->
       match_states (Returnstate s v m)
                    (Returnstate s' v' m')
   | match_states_interm:
       forall s sp pc rs m s' m' f r v'
-             (STACKS: match_stackframes m' (comp_of f) s s')
+             (STACKS: match_stackframes m' (* (comp_of f) *) s s')
              (MLD: Mem.extends m m'),
       is_return_spec f pc r ->
       f.(fn_stacksize) = 0 ->
       Val.lessdef (rs#r) v' ->
       match_states (State s f (Vptr sp Ptrofs.zero) pc rs m)
-                   (Returnstate s' v' m').
+                   (Returnstate s' v' m')
+  | match_states_state_fail: forall s f sp pc rs m r,
+      is_return_spec f pc r ->
+      f.(fn_stacksize) = 0 ->
+      match_states (State s f (Vptr sp Ptrofs.zero) pc rs m)
+                   (Failstate)
+  | match_states_return_fail: forall s v m,
+      match_states (Returnstate s v m)
+                   (Failstate)
+  | match_states_fail: forall s,
+      match_states Failstate s.
+
+
 
 (** The last case of [match_states] corresponds to the execution
   of a move/nop/return sequence in the original code that was
@@ -524,6 +537,7 @@ Definition measure (st: state) : nat :=
   | State s f sp pc rs m => (List.length s * (niter + 2) + return_measure f.(fn_code) pc + 1)%nat
   | Callstate s f args m => 0%nat
   | Returnstate s v m => (List.length s * (niter + 2))%nat
+  | Failstate => 0%nat
   end.
 
 Ltac TransfInstr :=
@@ -553,7 +567,11 @@ Proof.
 - (* nop *)
   TransfInstr. left. econstructor; split.
   eapply exec_Inop; eauto. constructor; auto.
-- (* eliminated nop *)
+- (* eliminated nop success *)
+  assert (s0 = pc') by congruence. subst s0.
+  right. split. simpl. omega. split. auto.
+  econstructor; eauto.
+- (* eliminated nop fail *)
   assert (s0 = pc') by congruence. subst s0.
   right. split. simpl. omega. split. auto.
   econstructor; eauto.
@@ -567,10 +585,14 @@ Proof.
   eapply exec_Iop; eauto.  rewrite <- EVAL'.
   apply eval_operation_preserved. exact symbols_preserved.
   econstructor; eauto. apply set_reg_lessdef; auto.
-- (* eliminated move *)
+- (* eliminated move success *)
   rewrite H1 in H. clear H1. inv H.
   right. split. simpl. omega. split. auto.
   econstructor; eauto. simpl in H0. rewrite PMap.gss. congruence.
+- (* eliminated move fail *)
+  rewrite H1 in H. clear H1. inv H.
+  right. split. simpl. omega. split. auto.
+  econstructor; eauto.
 
 - (* load *)
   TransfInstr.
@@ -635,7 +657,7 @@ Proof.
   rewrite comp_transl. eapply allowed_call_translated; eauto.
   rewrite comp_transl; eauto.
   constructor.
-  rewrite Efd. eapply match_stackframes_tail; eauto.
+  eapply match_stackframes_tail; eauto.
   (* TODO: Should be a lemma? *)
   { (* rewrite Efd. *)
     clear -FREE STACKS.
@@ -644,6 +666,7 @@ Proof.
     - constructor.
     - constructor; auto. eapply Mem.free_can_access_block_inj_1; eauto.
     - constructor; auto. }
+  unfold intra_compartment_call in INTRA.
     apply (cenv_compat_linkorder _ _ _ ORDER (compenv_program_compat _)).
   { red. simpl. congruence. }
   apply regs_lessdef_regs; auto.
@@ -694,7 +717,7 @@ Proof.
   rewrite comp_transl; eauto.
   constructor.
   (* TODO: Should be a lemma? *)
-  { rewrite COMP. clear -FREE STACKS.
+  { clear -FREE STACKS.
     revert STACKS. generalize (comp_of f). intros cp STACKS.
     induction STACKS.
     - constructor.
@@ -742,38 +765,78 @@ Proof.
   constructor; auto.
 
 - (* return *)
-  exploit Mem.free_parallel_extends; eauto. intros [m'1 [FREE EXT]].
+  (* case analysis*)
+  Require Import Classical.
+  destruct (classic (Genv.type_of_call tge (call_comp s') (comp_of f) = Genv.CrossCompartmentCall ->
+                     not_ptr (regmap_optget or Vundef rs'))).
++ exploit Mem.free_parallel_extends; eauto. intros [m'1 [FREE EXT]].
   TransfInstr.
   left. exists (Returnstate s' (regmap_optget or Vundef rs') m'1); split.
   eapply exec_Ireturn; eauto.
-  rewrite stacksize_preserved, comp_transl; eauto.
-  rewrite comp_transf_function. admit.
+  rewrite stacksize_preserved, comp_transl; eauto. eauto.
+  rewrite comp_transf_function. eauto.
   econstructor.
   (* (* rewrite comp_transf_function. *) constructor. *)
   (* TODO: Should be a lemma? *)
-  { admit. }
-    (* clear -FREE STACKS. *)
-    (* revert STACKS. generalize (comp_of f). intros cp STACKS. *)
-    (* induction STACKS. *)
-    (* - constructor. *)
-    (* - constructor; eauto. eapply Mem.free_can_access_block_inj_1; eauto. *)
-    (* - constructor; auto. } *)
+  { clear -FREE STACKS.
+    revert STACKS. generalize (comp_of f). intros cp STACKS.
+    induction STACKS.
+    - constructor.
+    - constructor; eauto. eapply Mem.free_can_access_block_inj_1; eauto.
+    - constructor; auto. }
   destruct or; simpl. apply RLD. constructor.
   auto.
++ exploit Mem.free_parallel_extends; eauto. intros [m'1 [FREE EXT]].
+  TransfInstr.
+  left. exists Failstate. split.
+  econstructor; eauto.
+  rewrite stacksize_preserved, comp_transl; eauto.
+  rewrite comp_transf_function. tauto.
+  constructor.
 
-- (* eliminated return None *)
+- (* eliminated return None success *)
   assert (or = None) by congruence. subst or.
   right. split. simpl. omega. split. auto.
   econstructor. eauto.
   simpl. constructor.
   eapply Mem.free_left_extends; eauto.
 
-- (* eliminated return Some *)
+- (* eliminated return Some success *)
   assert (or = Some r) by congruence. subst or.
   right. split. simpl. omega. split. auto.
   econstructor. eauto.
   simpl. auto.
   eapply Mem.free_left_extends; eauto.
+
+- (* eliminated return None fail *)
+  assert (or = None) by congruence. subst or.
+  right. split. simpl. omega. split. auto.
+  econstructor.
+
+- (* eliminated return Some fail *)
+  assert (or = Some r) by congruence. subst or.
+  right. split. simpl. omega. split. auto.
+  econstructor.
+
+- right. split. simpl. omega.
+  split. reflexivity.
+  constructor.
+
+- right. split. simpl. omega.
+  split. reflexivity.
+  constructor.
+
+- right. split. simpl. omega.
+  split. reflexivity.
+  constructor.
+
+- right. split. simpl. omega.
+  split. reflexivity.
+  constructor.
+
+- right. split. simpl. omega.
+  split. reflexivity.
+  constructor.
 
 - (* internal call *)
   exploit Mem.alloc_extends; eauto.
@@ -803,31 +866,38 @@ Proof.
 - (* external call *)
   exploit external_call_mem_extends; eauto.
   intros [res' [m2' [A [B [C D]]]]].
-  left. exists (Returnstate s' res' m2'); split.
+  destruct (classic (Genv.type_of_call tge (call_comp s') (comp_of ef) = Genv.CrossCompartmentCall ->
+                     not_ptr res')).
++ left. exists (Returnstate s' res' m2'); split.
   simpl. econstructor; eauto.
   eapply external_call_symbols_preserved; eauto. apply senv_preserved.
   destruct (needs_calling_comp (comp_of ef)) eqn:ALLOWED.
   { now rewrite <- (UPD ALLOWED). }
   exploit external_call_caller_independent; eauto.
-  admit.
   econstructor; eauto.
   (* TODO: Should be a lemma? *)
-  { admit. }
-  (* { clear -A H5. *)
-  (*   remember (call_comp s) as cp. clear Heqcp. unfold comp_of in H5; simpl in H5. *)
-  (*   induction H5. *)
-  (*   - constructor. *)
-  (*   - constructor; auto. eapply external_call_can_access_block; eauto. *)
-  (*   - constructor; auto. } *)
+  { clear -A H5.
+    remember (call_comp s) as cp. clear Heqcp. unfold comp_of in H5; simpl in H5.
+    induction H5.
+    - constructor.
+    - constructor; auto. eapply external_call_can_access_block; eauto.
+    - constructor; auto. }
++ left. exists Failstate. split.
+  econstructor; eauto.
+  eapply external_call_symbols_preserved; eauto. apply senv_preserved.
+  (* destruct (needs_calling_comp (comp_of ef)) eqn:ALLOWED. *)
+  (* { now rewrite <- (UPD ALLOWED). } *)
+  exploit external_call_caller_independent; eauto.
+  tauto.
+  constructor.
+
+- admit.
 
 - (* returnstate *)
   inv H2.
 + (* synchronous return in both programs *)
   left. econstructor; split.
   apply exec_return.
-  rewrite comp_transf_function, <- type_of_call_translated.
-  { intros G. specialize (NO_CROSS_PTR G).
-    inv H5; auto; contradiction. }
   constructor; auto. apply set_reg_lessdef; auto.
 + (* return instr in source program, eliminated because of tailcall *)
   right. split. unfold measure. simpl length.
@@ -837,7 +907,9 @@ Proof.
   split. auto.
   econstructor; eauto.
   rewrite Regmap.gss. auto.
-Qed.
+
+- admit.
+Admitted.
 
 Lemma transf_initial_states:
   forall st1, initial_state prog st1 ->
